<https://w3id.org/consolid#> rdf:type owl:Ontology ;
    owl:versionIRI <urn:absolute:0.0.1> ;
    <http://purl.org/dc/terms/contributor> "Erik Mannens" , "Jakob Beetz" , "Pieter Pauwels" ;
    <http://purl.org/dc/terms/creator> "Jeroen Werbrouck" ;
    <http://purl.org/dc/terms/issued> "2022-02-01T12:00:00"^^xsd:dateTime ;
    <http://purl.org/dc/terms/license> <https://creativecommons.org/licenses/by/1.0/> ;
    <http://purl.org/dc/terms/title> "consolid vocabulary" .

#    Object Properties

:aggregates rdf:type owl:ObjectProperty ;
    rdfs:comment "The consolid:Reference-s or other consolid:ReferenceCollection-s aggregated by this consolid:ReferenceCollection." ;
    rdfs:domain :ReferenceCollection ; 
    rdfs:label "aggregates" .

:hasSatellite rdf:type owl:ObjectProperty ;
    rdfs:domain <http://www.w3.org/ns/dcat#Dataset> ;
    rdfs:range :Satellite ;
    rdfs:label "has Satellite"@en .

:hasServiceRegistry rdf:type owl:ObjectProperty ;
    rdfs:subPropertyOf :hasRegistry ;
    rdfs:domain :PartialProject ;
    rdfs:range :ServiceRegistry ;
    rdfs:label "has service registry"@en .

:hasSparqlSatellite rdf:type owl:ObjectProperty ;
    rdfs:subPropertyOf :hasSatellite ;
    rdfs:range :SparqlSatellite ;
    rdfs:label "has SPARQL satellite"@en .
                    
:hasUpdate rdf:type owl:ObjectProperty ;
    rdfs:label "has update"@en ;
    rdfs:comment "The update of a body of an oa:Annotation, with a new rdf:value."@en .

#    Classes

:Project rdf:type owl:Class ;
    rdfs:subClassOf <http://www.w3.org/ns/dcat#Catalog> ;
    rdfs:comment "A ConSolid Project is a DCAT Catalog that resolves to a federated multi-model. It may be recursive, i.e. ConSolid Projects may 'aggregate' each other via dcat:dataset" ;
    rdfs:label "Project" .

:ProjectResource rdf:type owl:Class ;
    rdfs:subClassOf <http://www.w3.org/ns/dcat#Dataset> ;
    rdfs:comment "A Project Resource is a dcat:Dataset describing project information such as BIM models, project plans, etc." ;
    rdfs:label "Project Resource" .

:ValidationResource rdf:type owl:Class ;
    rdfs:subClassOf <http://www.w3.org/ns/dcat#Dataset> ;
    rdfs:comment "A Validation Resource is a dcat:Dataset describing a resource with the purpose of validation." ;
    rdfs:label "Validation Resource" .

:ReferenceRegistry rdf:type owl:Class ;
    rdfs:subClassOf <http://www.w3.org/ns/dcat#Dataset> ;
    rdfs:comment "A Reference Registry is a dcat:Dataset describing a resource containing Reference Collections (i.e. 'ConSolid linksets')." ;
    rdfs:label "Reference Registry" .

:ReferenceCollection rdf:type owl:Class ;
    rdfs:comment "A Reference Collection collects digital references of the same 'abstract' concept. It may be seen as the top-level identifier of this concept as well." ;
    rdfs:label "Reference Collection" .

:Reference rdf:type owl:Class ;
    rdfs:comment "A Reference is the digital manifestation of an abstract concept." ;
    rdfs:label "Reference" .

:ShapeCollection rdf:type owl:Class ;
    rdfs:subClassOf dcat:Catalog ;
    rdfs:comment "A Shape Collection is a DCAT Catalog exclusively containing shapes." ;
    rdfs:label "Shape Collection" .

:Satellite rdf:type owl:Class ;
    rdfs:subClassOf <http://www.w3.org/ns/dcat#DataService> ;
    rdfs:comment "A consolid:Satellite is a highly trusted service, connected to a limited set of Solid Pods, mostly just one. It may function as an alternative storage mechanism, providing specific access to (nested) ldp:Containers, dcat:Datasets, dcat:Catalogs or dcat:Distributions. Satellites can also be thought of as 'digital assistents' to a Pod, aiding in synchronisation, data management etc. When working on a Solid Pod, it must be able to check access rights." ;
    rdfs:label "Satellite" .

:SparqlSatellite rdf:type owl:Class ;
    rdfs:subClassOf :Satellite ;
    rdfs:comment "A SPARQL Satellite is a specifiic sort of satellite, mirroring RDF resources on the Pod and allowing to query their union with SPARQL. The satellite should check the access rights for every result it acquires." ;
    rdfs:label "SPARQL satellite" .

:RuntimeProperty rdf:type owl:Class ;
    rdfs:comment "A Runtime Property is a property that cannot be explicitly present in the data, but needs to be generated dynamically. E.g. when in order to conform to a specific shape, a dataset must refer to a project ID, but in ConSolid a dataset may be part of multiple projects. In this case, the project ID must be generated dynamically." ;
    rdfs:label "Runtime Property" .